01_Introduction.thy
@@ -5,15 +5,6 @@ theory "01_Introduction"
 begin
 (*>*)
 
-chapter \<open>QUESTIONS\<close>
-
-text\<open>
-  \begin{itemize}
-    \item How much explain the proofs? \\
-    \item How reference thm names? \\
-  \end{itemize}
-\<close>
-
 chapter\<open>Snippets\<close>
 
 section\<open>Earley\<close>
